src/theory/bir/bir_env_oldScript.sml
@@ -78,6 +78,19 @@ val bir_env_vars_are_initialised_EQ_envty = store_thm("bir_env_vars_are_initiali
   REWRITE_TAC [bir_env_vars_are_initialised_def, bir_envty_includes_vs_def, bir_env_var_is_initialised_EQ_envty]
 );
 
+(* ===================== *)
+
+(* TODO: This is used with get, for now. Rename to reflect this? *)
+Definition bir_ext_env_ext_is_valid_def:
+  bir_ext_env_ext_is_valid (ext_st:'ext_state_t) (ext_fn, ext_ty) <=>
+  ?v. bir_eval_extget ext_fn ext_ty ext_st = SOME v /\
+      type_of_bir_val v = ext_ty
+End
+
+Definition bir_ext_env_exts_are_valid_def:
+  bir_ext_env_exts_are_valid (ext_st:'ext_state_t) exts <=>
+  !ext_fn, ext_ty. (ext_fn, ext_ty) IN exts ==> bir_ext_env_ext_is_valid ext_st (ext_fn, ext_ty)
+End
 
 (* ===================== *)
 
@@ -237,6 +250,31 @@ REWRITE_TAC [bir_is_well_typed_env_THM]
 
 (* ===================== *)
 
+Theorem bir_ext_env_exts_are_valid_EMPTY:
+  !ext_st:'ext_state_t. bir_ext_env_exts_are_valid ext_st {}
+Proof
+fs [bir_ext_env_exts_are_valid_def, bir_ext_env_ext_is_valid_def, GSYM pairTheory.PFORALL_THM]
+QED
+
+Theorem bir_ext_env_exts_are_valid_UNION:
+  !ext_st:'ext_state_t exts1 exts2.
+  bir_ext_env_exts_are_valid ext_st (exts1 UNION exts2) <=>
+    (bir_ext_env_exts_are_valid ext_st exts1 /\
+     bir_ext_env_exts_are_valid ext_st exts2)
+Proof
+rpt strip_tac >>
+eq_tac >> (
+  rpt strip_tac
+) >> (
+  fs [bir_ext_env_exts_are_valid_def, bir_ext_env_ext_is_valid_def, GSYM pairTheory.PFORALL_THM]
+) >>
+rpt strip_tac >> (
+  metis_tac[]
+)
+QED
+
+(* ===================== *)
+
 val bir_var_set_is_well_typed_def = Define `bir_var_set_is_well_typed vs <=>
   (!v1 v2. (v1 IN vs /\ v2 IN vs /\ (bir_var_name v1 = bir_var_name v2)) ==>
            (bir_var_type v1 = bir_var_type v2))`;
@@ -268,7 +306,6 @@ val bir_var_set_is_well_typed_INSERT = store_thm ("bir_var_set_is_well_typed_INS
 
 SIMP_TAC std_ss [bir_var_set_is_well_typed_def, IN_INSERT] >>
 METIS_TAC[]);
-
 
 val bir_var_set_is_well_typed_UNION = store_thm ("bir_var_set_is_well_typed_UNION",
 ``!vs1 vs2. bir_var_set_is_well_typed (vs1 UNION vs2) <=>
